proof of non-interference, complete

coq/two/LambdaTwo.v
@@ -1,6 +1,14 @@
-Require Import Recdef Wf_nat.
+Require Import FunctionalExtensionality.
 Require Import LibTactics.
 Require Export LambdaTwoSyntax IndistinguishabilityTwo.
+
+Lemma functional_extensionality_ex :
+  forall {A : Type} (f g : A -> Prop),
+    (forall x, f x = g x) ->
+    (exists x, f x) = (exists x, g x).
+Proof.
+  intros. apply functional_extensionality in H. subst. reflexivity.
+Qed.
 
 Definition pair_lt (a b : nat * nat) : Prop :=
   fst a + snd a < fst b + snd b.
@@ -9,10 +17,10 @@ Lemma pair_lt_wf' :
   forall s a, fst a + snd a <= s -> Acc pair_lt a.
 Proof.
   induction s; intros a H1.
-  - destruct a as [a1 a2]; destruct a1; destruct a2; auto.
-    apply Acc_intro. intros y H2. inversion H2.
+  - destruct a as [a1 a2]; destruct a1; destruct a2;
+    apply Acc_intro; intros y H2; inversion H1; inversion H2.
   - inversion H1 as [H2 | n H2 Heq]; auto.
-    apply Acc_intro. intros y H3. inversion H3; auto.
+    apply Acc_intro. intros y H3. apply IHs. inversion H3; omega.
 Defined.
 
 Theorem pair_lt_wf : well_founded pair_lt.
@@ -25,13 +33,8 @@ Definition eval_kl : nat * nat -> two -> (value -> value -> Prop) ->
   refine
     (Fix pair_lt_wf (fun _ => two -> (value -> value -> Prop) ->
                               two -> env -> term -> atom -> Prop)
-         (fun (kl : nat * nat)
-              (eval_kl : forall kl' : nat * nat,
-                           pair_lt kl' kl ->
-                           two -> (value -> value -> Prop) ->
-                           two -> env -> term -> atom -> Prop) =>
-            fun (L : two) (P : value -> value -> Prop)
-                (pc : two) (e : env) (t : term) (a : atom) =>
+         (fun kl eval_kl =>
+            fun L P pc e t a =>
               match t with
                 | TBool b =>
                   a = Atom (VBool b) pc
@@ -46,11 +49,10 @@ Definition eval_kl : nat * nat -> two -> (value -> value -> Prop) ->
                 | TApp t1 t2 =>
                   if Compare_dec.zerop (fst kl) then False
                   else let eval := eval_kl (fst kl - 1, snd kl) _ in
-                       exists e1' t1' l1 a2 a3,
+                       exists e1' t1' l1 a2,
                          eval L P pc e t1 (Atom (VClos e1' t1') l1) /\
                          eval L P pc e t2 a2 /\
-                         eval L P l1 (a2 :: e1') t1' a3 /\
-                         a = a3
+                         eval L P l1 (a2 :: e1') t1' a
                 | TDecl t1 t2 =>
                   if Compare_dec.zerop (fst kl) then False
                   else let eval := eval_kl (fst kl - 1, snd kl) _ in
@@ -69,51 +71,98 @@ Definition eval_kl : nat * nat -> two -> (value -> value -> Prop) ->
   unfold pair_lt; simpl; omega.
 Defined.
 
-Definition eval (L : two) (P : value -> value -> Prop)
-           (pc : two) (e : env) (t : term) (a : atom) : Prop :=
-  exists k, forall l, eval_kl (k, l) L P pc e t a.
+Lemma eval_kl_eq :
+  forall kl,
+    eval_kl kl =
+    fun L P pc e t a =>
+      match t with
+        | TBool b =>
+          a = Atom (VBool b) pc
+        | TNat n =>
+          a = Atom (VNat n) pc
+        | TVar n =>
+          exists v l,
+            atIndex e n = Some (Atom v l) /\
+            a = Atom v (l ⊔ pc)
+        | TAbs t' =>
+          a = Atom (VClos e t') pc
+        | TApp t1 t2 =>
+          if Compare_dec.zerop (fst kl) then False
+          else let eval := eval_kl (fst kl - 1, snd kl) in
+               exists e1' t1' l1 a2,
+                 eval L P pc e t1 (Atom (VClos e1' t1') l1) /\
+                 eval L P pc e t2 a2 /\
+                 eval L P l1 (a2 :: e1') t1' a
+        | TDecl t1 t2 =>
+          if Compare_dec.zerop (fst kl) then False
+          else let eval := eval_kl (fst kl - 1, snd kl) in
+               exists e1' t1' l1 a2 v3 l3,
+                 eval L P pc e t1 (Atom (VClos e1' t1') l1) /\
+                 eval L P pc e t2 a2 /\
+                 eval L P l1 (a2 :: e1') t1' (Atom v3 l3) /\
+                 if bottomp l3 then a = Atom v3 Bottom2
+                 else let eval := eval_kl (snd kl, fst kl - 1) in
+                      (forall a2' e2' v3',
+                         env_LPequiv L P (a2 :: e1') (a2' :: e2') ->
+                         eval L P l1 (a2' :: e2') t1' (Atom v3' Top2) ->
+                         value_LPequiv L P v3 v3') /\
+                      a = Atom v3 Bottom2
+      end.
+Proof.
+  intro kl.
+  apply (Fix_eq pair_lt_wf (fun _ => two -> (value -> value -> Prop) ->
+                                     two -> env -> term -> atom -> Prop));
+    intros; destruct x as [x1 x2].
+  apply functional_extensionality; intro L.
+  apply functional_extensionality; intro P.
+  apply functional_extensionality; intro pc.
+  apply functional_extensionality; intro e.
+  apply functional_extensionality; intro t.
+  apply functional_extensionality; intro a.
+  destruct t; try reflexivity;
+  assert (H': forall (y : nat * nat), f y = g y) by
+      (intro; apply functional_extensionality; apply H).
+  - destruct x1; auto; simpl.
+    apply functional_extensionality_ex; intro e1'.
+    apply functional_extensionality_ex; intro t1'.
+    apply functional_extensionality_ex; intro l1.
+    apply functional_extensionality_ex; intro a2.
+    rewrite H'. reflexivity.
+  - destruct x1; auto; simpl.
+    apply functional_extensionality_ex; intro e1'.
+    apply functional_extensionality_ex; intro t1'.
+    apply functional_extensionality_ex; intro l1.
+    apply functional_extensionality_ex; intro a2.
+    apply functional_extensionality_ex; intro v3.
+    apply functional_extensionality_ex; intro l3.
+    destruct l3; rewrite H'; simpl; try rewrite H'; reflexivity.
+Qed.
 
 Lemma eval_kl_bool :
   forall k l L P pc e b,
     eval_kl (k, l) L P pc e (TBool b) (Atom (VBool b) pc).
-Proof.
-  introv. destruct k; destruct l; reflexivity.
-Qed.
+Proof. intros. rewrite eval_kl_eq. auto. Qed.
 
 Lemma eval_kl_bool_inv :
   forall k l L P pc e b a,
-    eval_kl (k, l) L P pc e (TBool b) a ->
-    a = Atom (VBool b) pc.
-Proof.
-  introv Heval.
-  destruct a as [v1 l1]; destruct v1 as [b1 | n1 | e1 t1];
-  destruct k; destruct l; inversion Heval; reflexivity.
-Qed.
+    eval_kl (k, l) L P pc e (TBool b) a -> a = Atom (VBool b) pc.
+Proof. intros. rewrite eval_kl_eq in H. auto. Qed.
 
 Lemma eval_kl_nat :
   forall k l L P pc e n,
     eval_kl (k, l) L P pc e (TNat n) (Atom (VNat n) pc).
-Proof.
-  introv. destruct k; destruct l; reflexivity.
-Qed.
+Proof. intros. rewrite eval_kl_eq. auto. Qed.
 
 Lemma eval_kl_nat_inv :
   forall k l L P pc e n a,
-    eval_kl (k, l) L P pc e (TNat n) a ->
-    a = Atom (VNat n) pc.
-Proof.
-  introv Heval.
-  destruct a as [v1 l1]; destruct v1 as [b1 | n1 | e1 t1];
-  destruct k; destruct l; inversion Heval; reflexivity.
-Qed.
+    eval_kl (k, l) L P pc e (TNat n) a -> a = Atom (VNat n) pc.
+Proof. intros. rewrite eval_kl_eq in H. auto. Qed.
 
 Lemma eval_kl_var :
   forall k l L P pc e n v' l',
     atIndex e n = Some (Atom v' l') ->
     eval_kl (k, l) L P pc e (TVar n) (Atom v' (l' ⊔ pc)).
-Proof.
-  introv He. destruct k; destruct l; exists v' l'; auto.
-Qed.
+Proof. intros. rewrite eval_kl_eq. exists v' l'. auto. Qed.
 
 Lemma eval_kl_var_inv :
   forall k l L P pc e n a,
@@ -121,28 +170,17 @@ Lemma eval_kl_var_inv :
     exists v' l',
       atIndex e n = Some (Atom v' l') /\
       a = Atom v' (l' ⊔ pc).
-Proof.
-  introv Heval.
-  destruct a as [v1 l1]; destruct v1 as [b1 | n1 | e1 t1];
-  destruct k; destruct l; inversion Heval; auto.
-Qed.
+Proof. intros. rewrite eval_kl_eq in H. auto. Qed.
 
 Lemma eval_kl_abs :
   forall k l L P pc e t',
     eval_kl (k, l) L P pc e (TAbs t') (Atom (VClos e t') pc).
-Proof.
-  introv. destruct k; destruct l; reflexivity.
-Qed.
-  
+Proof. intros. rewrite eval_kl_eq. auto. Qed.
+
 Lemma eval_kl_abs_inv :
-  forall k l L P pc e t' a,
-    eval_kl (k, l) L P pc e (TAbs t') a ->
-    a = Atom (VClos e t') pc.
-Proof.
-  introv Heval.
-  destruct a as [v1 l1]; destruct v1 as [b1 | n1 | e1 t1];
-  destruct k; destruct l; inversion Heval; reflexivity.
-Qed.
+  forall k l L P pc e t a,
+    eval_kl (k, l) L P pc e (TAbs t) a -> a = Atom (VClos e t) pc.
+Proof. intros. rewrite eval_kl_eq in H. auto. Qed.
 
 Lemma eval_kl_app :
   forall k l L P pc e t1 t2 e1' t1' l1 a2 a3,
@@ -151,21 +189,29 @@ Lemma eval_kl_app :
     eval_kl (k, l) L P l1 (a2 :: e1') t1' a3 ->
     eval_kl (S k, l) L P pc e (TApp t1 t2) a3.
 Proof.
-  (* TODO *)
-  Admitted.
+  intros.
+  rewrite eval_kl_eq. simpl.
+  replace (k - 0) with k by omega.
+  exists e1' t1' l1 a2. auto.
+Qed.
 
 Lemma eval_kl_app_inv :
   forall k l L P pc e t1 t2 a,
     eval_kl (k, l) L P pc e (TApp t1 t2) a ->
-    exists k' e1' t1' l1 a2 a3,
+    exists k' e1' t1' l1 a2,
       k = S k' /\
       eval_kl (k', l) L P pc e t1 (Atom (VClos e1' t1') l1) /\
       eval_kl (k', l) L P pc e t2 a2 /\
-      eval_kl (k', l) L P l1 (a2 :: e1') t1' a3 /\
-      a = a3.
+      eval_kl (k', l) L P l1 (a2 :: e1') t1' a.
 Proof.
-  (* TODO *)
-  Admitted.
+  intros.
+  rewrite eval_kl_eq in H.
+  destruct k; simpl in H.
+  - inversion H.
+  - destruct H as [e1' [t1' [l1 [a2 [H1 [H2 H3]]]]]].
+    replace (k - 0) with k in * by omega.
+    exists k e1' t1' l1 a2. auto.
+Qed.
 
 Lemma eval_kl_decl1 :
   forall k l L P pc e t1 t2 e1' t1' l1 a2 v3,
@@ -174,8 +220,11 @@ Lemma eval_kl_decl1 :
     eval_kl (k, l) L P l1 (a2 :: e1') t1' (Atom v3 Bottom2) ->
     eval_kl (S k, l) L P pc e (TDecl t1 t2) (Atom v3 Bottom2).
 Proof.
-  (* TODO *)
-  Admitted.
+  intros.
+  rewrite eval_kl_eq. simpl.
+  replace (k - 0) with k by omega.
+  exists e1' t1' l1 a2 v3 Bottom2. simpl. auto.
+Qed.
 
 Lemma eval_kl_decl2 :
   forall k l L P pc e t1 t2 e1' t1' l1 a2 v3,
@@ -188,8 +237,11 @@ Lemma eval_kl_decl2 :
        value_LPequiv L P v3 v3') ->
     eval_kl (S k, l) L P pc e (TDecl t1 t2) (Atom v3 Bottom2).
 Proof.
-  (* TODO *)
-  Admitted.
+  intros.
+  rewrite eval_kl_eq. simpl.
+  replace (k - 0) with k by omega.
+  exists e1' t1' l1 a2 v3 Top2. simpl. auto.
+Qed.
 
 Lemma eval_kl_decl_inv :
   forall k l L P pc e t1 t2 a,
@@ -211,5 +263,17 @@ Lemma eval_kl_decl_inv :
           value_LPequiv L P v3 v3') /\
        a = Atom v3 Bottom2).
 Proof.
-  (* TODO *)
-  Admitted.
+  intros.
+  rewrite eval_kl_eq in H.
+  destruct k; simpl in H.
+  - inversion H.
+  - destruct H as [e1' [t1' [l1 [a2 [v3 [l3 [H1 [H2 [H3 H4]]]]]]]]].
+    replace (k - 0) with k in * by omega.
+    destruct l3; simpl in H4.
+    + left. exists k e1' t1' l1 a2 v3. auto.
+    + right. exists k e1' t1' l1 a2 v3. auto.
+Qed.
+
+Definition eval (L : two) (P : value -> value -> Prop)
+           (pc : two) (e : env) (t : term) (a : atom) : Prop :=
+  exists k, forall l, eval_kl (k, l) L P pc e t a.
